chore: bump to nightly-2026-03-12

Tutorial/VCGen.lean
@@ -217,34 +217,6 @@ def nodup (l : List Int) : Bool := Id.run do
 :::
 
 ::::paragraph
-:::codeOnly
-```lean
--- NOTE: This is needed because a recent nightly didn't update the
--- type of Invariant.withEarlyReturn to use MProd
-abbrev withEarlyReturn {α} {xs : List α} {γ : Type (max u₁ u₂)}
-  (onContinue : List.Cursor xs → β → Assertion ps)
-  (onReturn : γ → β → Assertion ps)
-  (onExcept : ExceptConds ps := ExceptConds.false) :
-    Invariant xs (MProd (Option γ) β) ps :=
-  ⟨fun ⟨xs, x, b⟩ => spred(
-        (⌜x = none⌝ ∧ onContinue xs b)
-      ∨ (∃ r, ⌜x = some r⌝ ∧ ⌜xs.suffix = []⌝ ∧ onReturn r b)),
-   onExcept⟩
--- This test will fail when upstream has been fixed. At that time,
--- remove the helper and update the proof again.
-/--
-info:
-Std.Do.Invariant.withEarlyReturn.{u₁, u₂} {β : Type (max u₁ u₂)}
-  {ps : PostShape} {α : Type (max u₁ u₂)} {xs : List α}
-  {γ : Type (max u₁ u₂)} (onContinue : xs.Cursor → β → Assertion ps)
-  (onReturn : γ → β → Assertion ps)
-  (onExcept : ExceptConds ps := ExceptConds.false) :
-  Invariant xs (Option γ × β) ps
--/
-#guard_msgs (whitespace := lax) in
-#check Invariant.withEarlyReturn
-```
-:::
 
 This function is correct if it returns {name}`true` for every list that satisfies {name}`List.Nodup` and {name}`false` for every list that does not.
 Just as it was in {name}`mySum`, the use of {keywordOf Lean.Parser.Term.do}`do`-notation and the {name}`Id` monad is an internal implementation detail of {name}`nodup`.
@@ -255,7 +227,7 @@ theorem nodup_correct (l : List Int) : nodup l ↔ l.Nodup := by
   apply Id.of_wp_run_eq h
   mvcgen
   invariants
-  · withEarlyReturn
+  · Invariant.withEarlyReturn
       (onReturn := fun ret seen => ⌜ret = false ∧ ¬l.Nodup⌝)
       (onContinue := fun xs seen =>
         ⌜(∀ x, x ∈ seen ↔ x ∈ xs.prefix) ∧ xs.prefix.Nodup⌝)
